snapshots/hacl-c/Chacha20Poly1305.c
@@ -1,37 +1,97 @@
 #include "Chacha20Poly1305.h"
-void
-Hacl_AEAD_Chacha20Poly1305_encrypt(
+
+Prims_int Chacha20Poly1305_noncelen;
+
+Prims_int Chacha20Poly1305_keylen;
+
+Prims_int Chacha20Poly1305_maclen;
+
+uint32_t
+Chacha20Poly1305_aead_encrypt(
   uint8_t *c,
   uint8_t *mac,
   uint8_t *m,
-  uint64_t mlen,
+  uint32_t mlen,
   uint8_t *aad,
-  uint64_t aadlen,
-  uint8_t *n,
-  uint8_t *k
+  uint32_t aadlen,
+  uint8_t *k,
+  uint8_t *n
 )
 {
-  uint32_t ctx[16] = { 0 };
-  //uint32_t ctx[16] = { 0 };
-  Hacl_Symmetric_Chacha20_chacha_keysetup(ctx, k);
-  Hacl_Symmetric_Chacha20_chacha_ietf_ivsetup(ctx, n, 1);
-  Hacl_Symmetric_Chacha20_chacha_encrypt_bytes(ctx, m, c, mlen);
-
-  uint8_t mackey[32] = {0};
-  Hacl_Symmetric_Chacha20_chacha_keysetup(ctx, k);
-  Hacl_Symmetric_Chacha20_chacha_ietf_ivsetup(ctx, n, 0);
-  Hacl_Symmetric_Chacha20_chacha_encrypt_bytes(ctx, mackey, mackey, 64);
-
-  uint64_t buf[6] = { 0 };
-  uint64_t *r = buf;
-  uint64_t *h = buf + (uint32_t )3;
-  Hacl_Impl_Poly1305_64_poly1305_state st = { .x00 = r, .x01 = h };
-  Hacl_Impl_Poly1305_64_mac_blocks_init(st, c, mlen, mackey);
-  Hacl_Impl_Poly1305_64_mac_blocks_continue(st, aad, aadlen);
-  uint8_t last[16];
-  store64_le(last,aadlen);
-  store64_le(last+16,mlen);
-  Hacl_Impl_Poly1305_64_mac_blocks_finish(st, mac, last, 16, mackey);
-  
-  //Hacl_Impl_Poly1305_64_crypto_onetimeauth(mac, c, mlen, mackey);
+  Chacha20_chacha20(c, m, mlen, k, n, (uint32_t )1);
+  uint8_t b[64] = { 0 };
+  Chacha20_chacha20_key_block(b, k, n, (uint32_t )0);
+  uint8_t *mk = b;
+  uint8_t *key_s = mk + (uint32_t )16;
+  uint64_t buf[2];
+  Poly1305_64_state st;
+  st.x00 = buf;
+  st.x01 = buf+1;
+  uint8_t lb[16] = { 0 };
+  Poly1305_64_poly1305_blocks_init(st, aad, aadlen, mk);
+  Poly1305_64_poly1305_blocks_continue(st, c, mlen);
+  uint8_t *x0 = lb;
+  /* start inlining Hacl.Endianness.hstore64_le */
+  /* start inlining Hacl.Endianness.store64_le */
+  store64_le(x0, (uint64_t )aadlen);
+  /* end inlining Hacl.Endianness.store64_le */
+  /* end inlining Hacl.Endianness.hstore64_le */
+  uint8_t *x00 = lb + (uint32_t )8;
+  /* start inlining Hacl.Endianness.hstore64_le */
+  /* start inlining Hacl.Endianness.store64_le */
+  store64_le(x00, (uint64_t )mlen);
+  /* end inlining Hacl.Endianness.store64_le */
+  /* end inlining Hacl.Endianness.hstore64_le */
+  Poly1305_64_poly1305_blocks_finish(st, lb, mac, key_s);
+  return (uint32_t )0;
 }
+
+uint32_t
+Chacha20Poly1305_aead_decrypt(
+  uint8_t *m,
+  uint8_t *c,
+  uint32_t mlen,
+  uint8_t *mac,
+  uint8_t *aad,
+  uint32_t aadlen,
+  uint8_t *k,
+  uint8_t *n
+)
+{
+  uint8_t b[64] = { 0 };
+  Chacha20_chacha20_key_block(b, k, n, (uint32_t )0);
+  uint8_t *mk = b;
+  uint8_t *key_s = mk + (uint32_t )16;
+  uint8_t rmac[16] = { 0 };
+  uint64_t buf[2];
+  Poly1305_64_state st;
+  st.x00 = buf;
+  st.x01 = buf+1;
+  uint8_t lb[16] = { 0 };
+  Poly1305_64_poly1305_blocks_init(st, aad, aadlen, mk);
+  Poly1305_64_poly1305_blocks_continue(st, c, mlen);
+  uint8_t *x0 = lb;
+  /* start inlining Hacl.Endianness.hstore64_le */
+  /* start inlining Hacl.Endianness.store64_le */
+  store64_le(x0, (uint64_t )aadlen);
+  /* end inlining Hacl.Endianness.store64_le */
+  /* end inlining Hacl.Endianness.hstore64_le */
+  uint8_t *x00 = lb + (uint32_t )8;
+  /* start inlining Hacl.Endianness.hstore64_le */
+  /* start inlining Hacl.Endianness.store64_le */
+  store64_le(x00, (uint64_t )mlen);
+  /* end inlining Hacl.Endianness.store64_le */
+  /* end inlining Hacl.Endianness.hstore64_le */
+  Poly1305_64_poly1305_blocks_finish(st, lb, rmac, key_s);
+  uint8_t verify = Hacl_Policies_cmp_bytes(mac, rmac, (uint32_t )16);
+  uint32_t res;
+  if (verify == (uint8_t )0)
+  {
+    Chacha20_chacha20(m, c, mlen, k, n, (uint32_t )1);
+    res = (uint32_t )0;
+  }
+  else
+    res = (uint32_t )1;
+  return res;
+}
+
