code/poly1305/Poly1305_64.fst
@@ -7,11 +7,19 @@ open FStar.Seq
 open FStar.HyperStack
 open FStar.Endianness
 open FStar.Buffer
+open Hacl.Cast
 
 
+module H8   = Hacl.UInt8
+module Limb = Hacl.Bignum.Limb
+module Wide = Hacl.Bignum.Wide
+module U8   = FStar.UInt8
+module U32  = FStar.UInt32
 module U64  = FStar.UInt64
 module I = Hacl.Impl.Poly1305_64
 module S = Hacl.Spec.Poly1305_64
+module Poly = Hacl.Standalone.Poly1305_64
+       	      
 
 (* Type Aliases *)
 type uint8_p = Buffer.buffer Hacl.UInt8.t
@@ -43,6 +51,7 @@ val init:
 let init st k =
   let _ = I.poly1305_init_ st (Buffer.sub k 0ul 16ul) in ()
 
+let empty_log : I.log_t = Ghost.hide (Seq.createEmpty)
 
 val update_block:
   st:state ->
@@ -51,7 +60,7 @@ val update_block:
     (requires (fun h -> stable h st /\ live h m))
     (ensures  (fun h0 updated_log h1 -> modifies_1 (get_accumulator st) h0 h1 /\ stable h1 st))
 let update_block st m =
-  let _ = I.poly1305_update (FStar.Ghost.hide (Seq.createEmpty)) st m in ()
+  let _ = I.poly1305_update empty_log st m in ()
 
 
 #reset-options "--initial_fuel 0 --max_fuel 0 --z3rlimit 100"
@@ -90,7 +99,7 @@ val update_last:
     (requires (fun h -> stable h st /\ live h m))
     (ensures  (fun h0 _ h1 -> modifies_1 (get_accumulator st) h0 h1 /\ before_finish h1 st))
 let update_last st m len =
-  I.poly1305_update_last (FStar.Ghost.hide Seq.createEmpty) st (Buffer.sub m 0ul len) (Hacl.Cast.sint32_to_sint64 len)
+  I.poly1305_update_last empty_log st (Buffer.sub m 0ul len) (Hacl.Cast.sint32_to_sint64 len)
 
 
 val finish:
@@ -117,3 +126,82 @@ val crypto_onetimeauth:
          let key     = Hacl.Spec.Endianness.reveal_sbytes (as_seq h0 k) in
          mac == Spec.Poly1305.poly1305 message key)))
 let crypto_onetimeauth output input len k = Hacl.Standalone.Poly1305_64.crypto_onetimeauth output input len k
+
+#set-options "--lax"
+
+private val pad_16_bytes:
+  input:uint8_p ->
+  len:U32.t{length input = U32.v len /\ U32.v len < 16 /\ U32.v len > 0} ->
+  StackInline (uint8_p)
+    (requires (fun h -> live h input))
+    (ensures (fun h0 output h1 -> live h0 input /\ live h1 output /\ frameOf output = h1.tip
+      /\ modifies_0 h0 h1 /\ length output = 16
+      /\ (let o = as_seq h1 output in let i = as_seq h0 input in
+         o == Spec.Chacha20Poly1305.pad_16 i)))
+private let pad_16_bytes input len =
+  let h0 = ST.get() in
+  let b = Buffer.create (uint8_to_sint8 0uy) 16ul in
+  Buffer.blit input 0ul b 0ul len;
+  let h = ST.get() in
+  no_upd_lemma_0 h0 h input;
+  Seq.lemma_eq_intro (as_seq h input) (Seq.slice (as_seq h input) 0 (U32.v len));
+  Seq.lemma_eq_intro (Seq.slice (as_seq h b) (U32.v len) 16) (Seq.create (16 - U32.v len) (uint8_to_sint8 0uy));
+  Seq.lemma_eq_intro (as_seq h b) (Spec.Chacha20Poly1305.pad_16 (as_seq h0 input));
+  b
+
+val poly1305_blocks_init:
+  st:state ->
+  input:uint8_p{disjoint (get_key st) input /\ disjoint (get_accumulator st) input} ->
+  len:U32.t{U32.v len = length input} ->
+  k:uint8_p{length k = 32 /\ disjoint k (get_key st) /\ disjoint k (get_accumulator st)} ->
+  Stack unit
+    (requires (fun h -> live_state h st /\ live h input /\ live h k))
+    (ensures (fun h0 _ h1 -> live_state h1 st /\ live h0 input /\ live h0 k /\ modifies_2 (get_key st) (get_accumulator st) h0 h1))
+let poly1305_blocks_init st input len k =
+  let l = I.poly1305_init_ st (Buffer.sub k 0ul 16ul) in
+  let len_16 = U32.(len >>^ 4ul) in
+  let rem_16 = U32.(len &^ 4ul)  in
+  let l = Poly.poly1305_blocks l st (Buffer.sub input 0ul U32.(16ul *^ len_16)) (Int.Cast.uint32_to_uint64 len_16) in
+  if U32.(rem_16 =^ 0ul) then ()
+  else (
+    push_frame();
+    let b = pad_16_bytes (Buffer.offset input U32.(len -^ rem_16)) rem_16 in
+    let l = I.poly1305_update l st b in
+    pop_frame()
+  )
+
+
+
+val poly1305_blocks_continue:
+  st:state ->
+  input:uint8_p{disjoint (get_accumulator st) input} ->
+  len:U32.t{U32.v len = length input} ->
+  Stack unit
+    (requires (fun h -> live_state h st /\ live h input))
+    (ensures (fun h0 _ h1 -> live_state h1 st /\ live h0 input /\ modifies_1 (get_accumulator st) h0 h1))
+let poly1305_blocks_continue st input len =
+  let len_16 = U32.(len >>^ 4ul) in
+  let rem_16 = U32.(len &^ 4ul)  in
+  let l = Poly.poly1305_blocks empty_log st (Buffer.sub input 0ul U32.(16ul *^ len_16)) (Int.Cast.uint32_to_uint64 len_16) in
+  if U32.(rem_16 =^ 0ul) then ()
+  else (
+    push_frame();
+    let b = pad_16_bytes (Buffer.offset input U32.(len -^ rem_16)) rem_16 in
+    let _ = I.poly1305_update l st b in
+    pop_frame()
+  )
+
+val poly1305_blocks_finish:
+  st:state ->
+  input:uint8_p{disjoint (get_accumulator st) input} ->
+  mac:uint8_p{disjoint (get_accumulator st) mac /\ disjoint mac input} ->
+  key_s:uint8_p{disjoint key_s (get_accumulator st) /\ disjoint key_s mac} ->
+  Stack unit
+    (requires (fun h -> live_state h st /\ live h input /\ live h mac))
+    (ensures (fun h0 _ h1 -> live h0 input /\ modifies_2 mac (get_accumulator st) h0 h1 /\ live h1 mac))
+let poly1305_blocks_finish st input mac key_s =
+  let _ = I.poly1305_update empty_log st input in
+  let _ = I.poly1305_update_last empty_log st (Buffer.offset input 16ul) 0uL in
+  let _ = I.poly1305_finish st mac key_s in
+  ()
+
