code/salsa-family/interfaces/Chacha20.fsti
@@ -7,6 +7,7 @@ open Hacl.Cast
 open Hacl.UInt32
 open FStar.Buffer
 open Hacl.Spec.Symmetric.Chacha20
+open Hacl.Spec.Endianness
 
 module U32 = FStar.UInt32
 module H8  = Hacl.UInt8
@@ -15,35 +16,30 @@ module H32 = Hacl.UInt32
 let u32 = U32.t
 let h32 = H32.t
 let uint8_p = buffer H8.t
-type chacha_ctx = b:Buffer.buffer h32{length b = 16}
 
-(* aligned to LibSodium API *) 
 
-(* sets the lower 12 words of the state (usable for multiple encryptions) *)
-val chacha_keysetup:
-  ctx:chacha_ctx ->
-  k:uint8_p{length k = 32 /\ disjoint ctx k} ->
+val chacha20_key_block:
+  block:uint8_p{length block = 64} ->
+  k:uint8_p{length k = 32 /\ disjoint block k} ->
+  n:uint8_p{length k = 12 /\ disjoint block n} ->
+  ctr:UInt32.t ->
   Stack unit
-    (requires (fun h -> live h ctx /\ live h k))
-    (ensures  (fun h0 _ h1 -> live h0 ctx /\ live h0 k /\ live h1 ctx /\ modifies_1 ctx h0 h1
-      /\ as_seq h1 ctx == chacha_keysetup_spec (as_seq h0 ctx) (as_seq h0 k)))
+    (requires (fun h -> live h block /\ live h k))
+    (ensures (fun h0 _ h1 -> live h1 block /\ modifies_1 block h0 h1))
 
-(* sets the upper 4 words of the state to a specific IV and counter *)
-val chacha_ietf_ivsetup:
-  ctx:chacha_ctx ->
-  k:uint8_p{length k = 12 /\ disjoint ctx k} ->
-  counter:u32 ->
+val chacha20:
+  output:uint8_p ->
+  plain:uint8_p{disjoint output plain} ->
+  len:U32.t{U32.v len = length output /\ U32.v len = length plain} ->
+  key:uint8_p{length key = 32} ->
+  nonce:uint8_p{length key = 12} ->
+  ctr:U32.t{U32.v ctr + (length plain / 64) < pow2 32} ->
   Stack unit
-    (requires (fun h -> live h ctx /\ live h k))
-    (ensures  (fun h0 _ h1 -> live h1 ctx /\ live h0 ctx /\ live h0 k /\ modifies_1 ctx h0 h1 
-      /\ as_seq h1 ctx == chacha_ietf_ivsetup_spec (as_seq h0 ctx) (as_seq h0 k) counter))
-
-(* encrypts len bytes from m to c [still missing full spec; the state is destroyed] *)
-val chacha_encrypt_bytes:
-  ctx:chacha_ctx ->
-  m:uint8_p ->
-  c:uint8_p{disjoint ctx c} ->
-  len:UInt32.t{U32.v len <= length m /\ U32.v len <= length c} ->
-  Stack unit
-    (requires (fun h -> live h c /\ live h m /\ live h ctx))
-    (ensures  (fun h0 _ h1 -> live h1 c /\ modifies_2 ctx c h0 h1))
+    (requires (fun h -> live h output /\ live h plain))
+    (ensures (fun h0 _ h1 -> live h1 output /\ live h0 plain /\ modifies_1 output h0 h1
+      /\ (let o = reveal_sbytes (as_seq h1 output) in
+         let plain = reveal_sbytes (as_seq h0 plain) in
+         let k = reveal_sbytes (as_seq h0 key) in
+         let n = reveal_sbytes (as_seq h0 nonce) in
+         let ctr = U32.v ctr in
+         o == Spec.CTR.counter_mode Spec.Chacha20.chacha20_ctx Spec.Chacha20.chacha20_cipher k n ctr plain)))
