code/poly1305/interfaces/Poly1305_64.fsti
@@ -9,6 +9,7 @@ open FStar.Endianness
 open FStar.Buffer
 
 
+module U32  = FStar.UInt32
 module U64  = FStar.UInt64
 
 
@@ -95,3 +96,29 @@ val crypto_onetimeauth:
          let message = Hacl.Spec.Endianness.reveal_sbytes (as_seq h0 input) in
          let key     = Hacl.Spec.Endianness.reveal_sbytes (as_seq h0 k) in
          mac == Spec.Poly1305.poly1305 message key)))
+
+val poly1305_blocks_init:
+  st:state ->
+  input:uint8_p{disjoint (get_key st) input /\ disjoint (get_accumulator st) input} ->
+  len:U32.t{U32.v len = length input} ->
+  k:uint8_p{length k = 32 /\ disjoint k (get_key st) /\ disjoint k (get_accumulator st)} ->
+  Stack unit
+    (requires (fun h -> live_state h st /\ live h input /\ live h k))
+    (ensures (fun h0 _ h1 -> live_state h1 st /\ live h0 input /\ live h0 k /\ modifies_2 (get_key st) (get_accumulator st) h0 h1))
+
+val poly1305_blocks_continue:
+  st:state ->
+  input:uint8_p{disjoint (get_accumulator st) input} ->
+  len:U32.t{U32.v len = length input} ->
+  Stack unit
+    (requires (fun h -> live_state h st /\ live h input))
+    (ensures (fun h0 _ h1 -> live_state h1 st /\ live h0 input /\ modifies_1 (get_accumulator st) h0 h1))
+
+val poly1305_blocks_finish:
+  st:state ->
+  input:uint8_p{disjoint (get_accumulator st) input} ->
+  mac:uint8_p{disjoint (get_accumulator st) mac /\ disjoint mac input} ->
+  key_s:uint8_p{disjoint key_s (get_accumulator st) /\ disjoint key_s mac} ->
+  Stack unit
+    (requires (fun h -> live_state h st /\ live h input /\ live h mac))
+    (ensures (fun h0 _ h1 -> live h0 input /\ modifies_2 mac (get_accumulator st) h0 h1 /\ live h1 mac))
